examples/sampler/verif_sampler_ingress_parser.v
@@ -20,17 +20,8 @@ Definition p := ["pipe"; "ingress_parser"].
 
 Open Scope func_spec.
 
-Definition tofino_parser_start_fundef :=
-  ltac:(get_fd ["TofinoIngressParser"; "start"] ge).
-
-Definition tofino_parser_resubmit_fundef :=
-  ltac:(get_fd ["TofinoIngressParser"; "parse_resubmit"] ge).
-
 Definition tofino_parser_port_metadata_fundef :=
   ltac:(get_fd ["TofinoIngressParser"; "parse_port_metadata"] ge).
-
-Definition test :=
-  ltac:(get_fd ["TofinoIngressParser"; "accept"] ge).
 
 Definition tofino_parser_port_metadata_spec: func_spec :=
   WITH,
@@ -60,6 +51,126 @@ Proof.
   step.
   entailer.
 Qed.
+
+#[export] Hint Extern 5 (func_modifies _ _ _ _ _) => (apply tofino_parser_port_metadata_body) : func_specs.
+
+Definition tofino_parser_resubmit_fundef :=
+  ltac:(get_fd ["TofinoIngressParser"; "parse_resubmit"] ge).
+
+Definition tofino_parser_resubmit_spec: func_spec :=
+  WITH,
+    PATH p
+    MOD None [["packet_in"]]
+    WITH (pin: packet_in) (_: 64 < Zlength pin) (_: False),
+      PRE
+        (ARG []
+        (MEM []
+        (EXT [ExtPred.singleton ["packet_in"] (ObjPin pin)])))
+      POST
+        (ARG_RET [] ValBaseNull
+        (MEM []
+           (EXT [ExtPred.singleton ["packet_in"] (ObjPin (skipn 64 pin))]))).
+
+Lemma tofino_parser_resubmit_body:
+  func_sound ge tofino_parser_resubmit_fundef nil
+    tofino_parser_resubmit_spec.
+Proof.
+  start_function.
+  step_call (@packet_in_advance_body Info);
+    [ entailer; instantiate (1 := 64); apply sval_refine_refl |
+      lia | assumption | ].
+  step_call (parser_reject_body ge ge); [entailer | assumption |].
+  step. entailer.
+Qed.
+
+#[export] Hint Extern 5 (func_modifies _ _ _ _ _) => (apply tofino_parser_resubmit_body) : func_specs.
+
+Definition tofino_parser_start_fundef :=
+  ltac:(get_fd ["TofinoIngressParser"; "start"] ge).
+
+Definition iimt_repr_sval (flag version port stamp: Z): Sval :=
+  ValBaseHeader
+    [("resubmit_flag", P4Bit 1 flag);
+     ("_pad1", P4Bit 1 0);
+     ("packet_version", P4Bit 2 version);
+     ("_pad2", P4Bit 3 0);
+     ("ingress_port", P4Bit 9 port);
+     ("ingress_mac_tstamp", P4Bit 48 stamp)] (Some true).
+
+Definition P4BitV (w : N) (v : Z) : Val :=
+  ValBaseBit (P4Arith.to_lbool w v).
+
+Definition iimt_repr_val (flag version port stamp: Z) : Val :=
+  ValBaseHeader
+    [("resubmit_flag", P4BitV 1 flag);
+     ("_pad1", P4BitV 1 0);
+     ("packet_version", P4BitV 2 version);
+     ("_pad2", P4BitV 3 0);
+     ("ingress_port", P4BitV 9 port);
+     ("ingress_mac_tstamp", P4BitV 48 stamp)] true.
+
+Definition tofino_parser_start_spec: func_spec :=
+  WITH,
+    PATH p
+    MOD None [["packet_in"]]
+    WITH (pin: packet_in) ver port stamp pin'
+         (_: extract ingress_intrinsic_metadata_t pin =
+             Some (iimt_repr_val 0 ver port stamp, SReturnNull, pin'))
+         (_: 64 < Zlength pin'),
+      PRE
+        (ARG []
+        (MEM []
+        (EXT [ExtPred.singleton ["packet_in"] (ObjPin pin)])))
+      POST
+        (ARG_RET [] ValBaseNull
+        (MEM []
+           (EXT [ExtPred.singleton ["packet_in"] (ObjPin (skipn 64 pin'))]))).
+
+Lemma tofino_parser_start_body:
+  func_sound ge tofino_parser_start_fundef nil
+    tofino_parser_start_spec.
+Proof.
+  start_function.
+  - step_call (@packet_in_extract_body Info); [entailer | apply H |].
+    step_if.
+    + simpl get in H1. exfalso; auto.
+    + simpl Ops.eval_cast in H1.
+      simpl get in H1. simpl build_abs_unary_op in H1.
+      unfold build_abs_unary_op in H1. simpl eval_sval_to_val in H1.
+      simpl in H1. exfalso. assumption.
+  - apply func_modifies_internal.
+    apply Forall_nil.
+    simple apply @block_modifies_cons.
+    + eauto 300 with nocore modifies.
+    + simple apply @block_modifies_cons.
+      simple apply @stmt_modifies_if.
+      simple eapply @stmt_modifies_method_call.
+      simple eapply @call_modifies_func; try eauto 300 with nocore modifies.
+      simpl.
+(*
+ simple eapply @stmt_modifies_assign
+ simple eapply @stmt_modifies_assign_call
+ simple apply @eq_refl
+ simple eapply @call_modifies_func
+ simple apply @eq_refl
+ (*external*) reflexivity
+ (*external*) (apply Forall2_cons)
+ simple apply @out_arg_In_vars_in
+ (*external*) (apply Forall2_nil)
+ (*external*) reflexivity
+
+ (*external*) (eapply func_modifies_frame; only 1: solve
+                            [ eauto  15 with nocore func_specs ])
+ (*external*) (apply incl_vars_None_None)
+ (*external*) (apply Forall_cons)
+ (*external*) reflexivity
+ (*external*) (apply Forall_nil)
+ (*external*) reflexivity
+
+ (*external*) (apply In_vars_Some)
+ simple apply in_eq
+ simple apply @block_modifies_nil *)
+Abort.
 
 Definition parser_start_fundef :=
   ltac:(get_fd ["SwitchIngressParser"; "start"] ge).
